pulse/test/Goto.fst
@@ -1,0 +1,39 @@
+module Goto
+open Pulse
+open Pulse.Lib.WithPure
+#lang-pulse
+
+fn test1 (r: ref int)
+    preserves live r
+{
+  {
+    goto fail;
+    label fail:
+  }
+}
+
+fn find_zero (a: array int) (sz: SizeT.t)
+  preserves pts_to a #'r 'va
+  requires with_pure (SizeT.v sz <= Seq.length 'va)
+  returns i: SizeT.t
+  ensures pure (SizeT.v i <= SizeT.v sz /\
+    (forall (j: nat). j < SizeT.v i ==> Seq.index 'va j <> 0))
+  ensures pure (SizeT.v i < SizeT.v sz ==> Seq.index 'va (SizeT.v i) == 0)
+{{
+  let mut i: SizeT.t = 0sz;
+  while (!i `SizeT.lt` sz)
+    invariant live i
+    invariant pure (SizeT.v !i <= SizeT.v sz /\
+      (forall (j: nat). j < SizeT.v (!i) ==> Seq.index 'va j <> 0))
+  {
+    with vi. assert i |-> vi;
+    if (a.(!i) = 0)
+      ensures pts_to a #'r 'va ** i |-> vi ** pure (Seq.index 'va (SizeT.v vi) <> 0)
+    {
+      goto return (!i);
+    };
+    i := !i `SizeT.add` 1sz;
+  };
+  !i
+  label return:
+}}
